proof/invariant-abstract/AARCH64/ArchSchedule_AI.thy
@@ -37,8 +37,8 @@ lemma arch_stt_tcb [wp,Schedule_AI_assms]:
   "arch_switch_to_thread t' \<lbrace>tcb_at t'\<rbrace>"
   by (wpsimp simp: arch_switch_to_thread_def wp: tcb_at_typ_at)
 
-lemma arch_stt_runnable[Schedule_AI_assms]:
-  "arch_switch_to_thread t \<lbrace>st_tcb_at runnable t\<rbrace>"
+lemma arch_stt_st_tcb_at[Schedule_AI_assms]:
+  "arch_switch_to_thread t \<lbrace>st_tcb_at Q t\<rbrace>"
   by (wpsimp simp: arch_switch_to_thread_def)
 
 lemma idle_strg:
@@ -86,28 +86,19 @@ lemma stit_activatable[Schedule_AI_assms]:
                  elim!: pred_tcb_weaken_strongerE)
   done
 
-lemma stt_invs [wp,Schedule_AI_assms]:
-  "switch_to_thread t' \<lbrace>invs\<rbrace>"
-  apply (simp add: switch_to_thread_def)
-  apply wp
-     apply (simp add: trans_state_update[symmetric] del: trans_state_update)
-    apply (rule_tac Q'="\<lambda>_. invs and tcb_at t'" in hoare_strengthen_post, wp)
-    apply (clarsimp simp: invs_def valid_state_def valid_idle_def
-                          valid_irq_node_def valid_machine_state_def)
-    apply (fastforce simp: cur_tcb_def obj_at_def
-                     elim: valid_pspace_eqI ifunsafe_pspaceI)
-   apply wp+
-  apply clarsimp
-  apply (simp add: is_tcb_def)
-  done
-end
+crunch set_vm_root, vcpu_switch
+  for scheduler_action[wp]: "\<lambda>s. P (scheduler_action s)"
+  (wp: crunch_wps simp: crunch_simps)
 
-interpretation Schedule_AI_U?: Schedule_AI_U
-proof goal_cases
-  interpret Arch .
-  case 1 show ?case
-    by (intro_locales; (unfold_locales; fact Schedule_AI_assms)?)
-qed
+lemma arch_stt_scheduler_action [wp, Schedule_AI_assms]:
+  "\<lbrace>\<lambda>s. P (scheduler_action s)\<rbrace> arch_switch_to_thread t' \<lbrace>\<lambda>_ s. P (scheduler_action s)\<rbrace>"
+  by (wpsimp simp: arch_switch_to_thread_def)
+
+lemma arch_stit_scheduler_action [wp, Schedule_AI_assms]:
+  "\<lbrace>\<lambda>s. P (scheduler_action s)\<rbrace> arch_switch_to_idle_thread \<lbrace>\<lambda>_ s. P (scheduler_action s)\<rbrace>"
+  by (wpsimp simp: arch_switch_to_idle_thread_def)
+
+end
 
 interpretation Schedule_AI?: Schedule_AI
 proof goal_cases
